ModularEngine/src/LogicEngine.FStar/types.fst
@@ -12,12 +12,10 @@
 *)
 
 module Types
-(* open TypeHeaders *)
+  open Crypto
   type principal = string
   type substrate = unit
   type ISubstrateUpdateTerm
-
-  (*val get_substrate : unit -> substrate*)
 
   extern reference Generics {language="F#";
                              dll="mscorlib";
@@ -26,113 +24,94 @@ module Types
   extern Generics type Dictionary :: * => * => *
   extern Generics type HashSet :: * => *
 
-  type typ =  (* IType *)
-  (* from Types.fs, see also Ast/ActivePatterns.fs *)
-  (* BasicType types *)
-    | Infon : typ
-    | Principal : typ
+  type typ =  (* IType *)  (* from Types.fs, see also Ast/ActivePatterns.fs *)
+    | Infon           : typ
+    | Principal       : typ
     | SubstrateUpdate : typ (* see ISubstrateUpdate.fs *)
-    | SubstrateQuery : typ (* see ISubstrateQuery.fs *)
-    | Action : typ
-    | Condition : typ
-    | RuleT : typ
-    | Evidence : typ
-  (* Substrate types *)
-    | Boolean : typ
-    | Int32 : typ
-    | Double : typ
-    | String : typ
+    | SubstrateQuery  : typ (* see ISubstrateQuery.fs *)
+    | Action          : typ
+    | Condition       : typ
+    | RuleT           : typ
+    | Evidence        : typ
+    | Boolean         : typ
+    | Int32           : typ
+    | BytesT          : typ
+    | Double          : typ
+    | String          : typ
 
   type var = (* IVar *)
-    { name : string; typ : typ }
+      { name : string; typ : typ }
   type vars = list var
 
   type constant =
-    | TrueT : constant
-    | FalseT : constant
-    | Int : int -> constant
+    | TrueT             : constant
+    | FalseT            : constant
+    | Int               : int -> constant
+    | Bytes             : bytes -> constant
     | SubstrateConstant : constant -> constant
     | PrincipalConstant : principal -> constant
 
-  type relationInfon = (* form TreeTerm.fs, def of type Function *)
-    { fname : string; 
-      retType: typ; 
-      argsType : list typ; 
-      identity : option term  }
-
+  type relationInfon = (* from TreeTerm.fs, def of type Function *)
+      { fname    : string; 
+        retType  : typ; 
+        argsType : list typ; 
+        identity : option term }
+        
   and func =
-  (* from Ast.Infon/ActivePatterns.fs *)
-  (* types from Ast.Infon/Primitives.fs, function SolveFunction *)
-  (* and its use in Ast.Infon/Builders.fs *)
-    (* Rule: <condition> do <action> *)
-    | SeqRule : func (* [RuleT;...; RuleT] -> RuleT *)
-    | EmptyRule : func (* [] -> RuleT *)
-    | Rule : func (* [Condition; Action] -> RuleT *)
-    | RuleOnce : func (* [Condition; Action] -> RuleT *)
-    (* Condition *)
-    | SeqCondition : func (* [Condition;...; Condition] -> Condition *)
-    | EmptyCondition : func (* [] -> Condition *)
-    | WireCondition : func (* [Infon; Principal] -> Condition *)
-      (* upon in concrete syntax *)
-    | KnownCondition : func (* [Infon] -> Condition *)
-      (* if in concrete syntax *)
-    (* Action *)
-    | SeqAction : func (* [Action;...; Action] -> Action *)
-    | EmptyAction : func (* [] -> Action *)
-    | Send : func (* [Principal; Infon] -> Action *)
-      (* ppal (destination), msg *)
-    | JustifiedSend : func (* [Principal; Infon] -> Action *)
-      (* ppal (destination), msg *)
-    | JustifiedSay : func (* [Principal; Infon] -> Action *)
-      (* ppal (destination), msg *)
-    | Learn : func (* [Infon] -> Action *)
-    | Forget : func (* [Infon] -> Action *)
-    | Install : func (* [RuleT] -> Action *)
-      (* add a rule to set of rules *)
-    | Uninstall : func (* [RuleT] -> Action *)
-    | Apply : func (* [SubstrateUpdate] -> Action *)
-      (* of substrateUpdateTerm // apply this update to the substrate *)
-    | Drop : func (* [Infon] -> Action *)
-      (* regarding an infon that came in as a message *)
-    (* Infon *)
-    | EmptyInfon : func (* [] -> Infon *)
-    | AsInfon : func (* [SubstrateQuery] -> Infon *)(* of substrateQueryTerm *)
-    | AndInfon : func (* [Infon; ...; Infon] -> Infon *)
-      (* may be easier to consider just binary case *)
-    | ImpliesInfon : func (* [Infon; Infon] -> Infon *)
-    | SaidInfon : func (* [Principal; Infon] -> Infon *)
-      (* ppal (sender), msg *)
-    | JustifiedInfon : func (* [Infon; Evidence] -> Infon *)
-    (* Evidence *)
-    | EmptyEvidence : func (* [] -> Evidence *)
-    | SignatureEvidence : func (* [Principal; Infon; Int32] -> Evidence *)
-      (* ppal, term, int *)
-      (* might want to change the third type to dsig, signature for .Net *)
-    | ModusPonensEvidence : func (* [Evidence; Evidence] -> Evidence *)
-    | AndEvidence : func (* [Evidence;... ; Evidence] -> Evidence *)
-    | AsInfonEvidence : func (* [SubstrateQuery] -> Evidence *)
-      (* of substrateQueryTerm *)
-    (* Relations defined by the writer of the policy *)
-    | RelationInfon (*of relationInfon*) : relationInfon -> func
-      (* no active pattern for it, base case for infons *)
+    | EmptyInfon    : func (* [] -> Infon *)
+    | AsInfon       : func (* [SubstrateQuery] -> Infon *)
+    | AndInfon      : func (* [Infon; ...; Infon] -> Infon *)
+    | ImpliesInfon  : func (* [Infon; Infon] -> Infon *)
+    | SaidInfon     : func (* [Principal; Infon] -> Infon *)
+    | JustifiedInon : func (* [Principal; Infon; Bytes] -> Infon *)
+    | RelationInfon : relationInfon -> func
+(* --- We should get rid of these remaining ones --- *)
+    | SeqRule : func 
+    | SeqCondition : func 
+    | SeqAction : func
+    | AndInfon : func 
+    | AndEvidence : func
+    | EmptyRule : func 
+    | Rule : func 
+    | RuleOnce : func
+    | EmptyCondition : func 
+    | WireCondition : func 
+    | KnownCondition : func
+    | EmptyAction : func 
+    | Send : func 
+    | JustifiedSend : func
+    | JustifiedSay : func 
+    | Learn : func 
+    | Forget : func
+    | Install : func 
+    | Uninstall : func
+    | Apply : func 
+    | Drop : func 
+    | EmptyInfon : func
+    | AsInfon : func 
+    | ImpliesInfon : func
+    | SaidInfon : func 
+    | JustifiedInfon : func
+    | EmptyEvidence : func 
+    | SignatureEvidence : func
+    | ModusPonensEvidence : func
+    | AsInfonEvidence : func 
 
   and ISubstrateQueryTerm::* = {n:term; low: term; hi: term}
 
   and term = (* ITerm *)
-  (* from Ast.Tree/ActivePatterns.fs *)
-  (* from Ast/ActivePatterns.fs *)
-    | Var : var -> term
-    | Const : constant -> term
-    | SubstrateQueryTerm : ISubstrateQueryTerm -> term
+    | Var                 : var -> term
+    | Const               : constant -> term
+    | App                 : func -> list term -> term
+    | SubstrateQueryTerm  : ISubstrateQueryTerm -> term
     | SubstrateUpdateTerm : ISubstrateUpdateTerm -> term
-    | App : func -> list term -> term
 
   and polyterm = 
-    | MonoTerm : term -> polyterm
-    | ForallT : vars -> term -> polyterm
+    | MonoTerm      : term -> polyterm
+    | ForallT       : vars -> term -> polyterm
+    | JustifiedPoly : term -> polyterm -> term -> polyterm
 
   type SubstrateSays :: substrate => ISubstrateQueryTerm => E
-
   val mkSubstrateQuery: term -> term -> term -> ISubstrateQueryTerm
   let mkSubstrateQuery i l h = {n=i; low=l; hi=h}
 
@@ -151,7 +130,6 @@ module Types
   type Knows :: polyterm => E
   type kpolyterm = i:polyterm{Knows i}
   type infostrate = list polyterm
-(*   type infostrate = list polyterm *)
   type prefix = list term
 
   type substitution = list (var * term)
